fstar/MLS.TreeDEM.Message.Framing.fst
@@ -12,228 +12,98 @@ open MLS.Result
 
 module NT = MLS.NetworkTypes
 
-noeq type message_plaintext (bytes:Type0) {|bytes_like bytes|} = {
-  content: message_content bytes;
-  auth: message_auth bytes;
-  membership_tag: option bytes;
-}
-
-noeq type message_ciphertext (bytes:Type0) {|bytes_like bytes|} = {
-  group_id: bytes;
-  epoch: nat;
-  content_type: content_type_nt;
-  authenticated_data: bytes;
-  encrypted_sender_data: bytes;
-  ciphertext: bytes;
-}
-
-noeq type message_ciphertext_content (bytes:Type0) {|bytes_like bytes|} (content_type:content_type_nt) = {
-  content: message_bare_content bytes content_type;
-  auth: message_auth bytes;
-  padding: list zero_byte;
-}
-
-noeq type encrypted_sender_data_content (bytes:Type0) {|bytes_like bytes|} = {
-  leaf_index: nat;
-  generation: nat;
-  reuse_guard: lbytes bytes 4;
-}
-
-(*** From/to network ***)
-
-val network_to_message_plaintext: #bytes:Type0 -> {|bytes_like bytes|} -> mls_plaintext_nt bytes -> result (message_plaintext bytes)
-let network_to_message_plaintext #bytes #bl pt =
-  content <-- network_to_message_content (WF_mls_plaintext ()) pt.content;
-  auth <-- network_to_message_auth pt.auth;
-  let membership_tag: option bytes =
-    if NT.S_member? pt.content.sender then (
-      Some pt.membership_tag
-    ) else None
-  in
-  return ({
-    content;
-    auth;
-    membership_tag;
-  } <: message_plaintext bytes)
-
-val message_plaintext_to_network: #bytes:Type0 -> {|bytes_like bytes|} -> message_plaintext bytes -> result (mls_plaintext_nt bytes)
-let message_plaintext_to_network #bytes #bl pt =
-  content <-- message_content_to_network pt.content;
-  auth <-- message_auth_to_network pt.auth;
-  if not ((NT.S_member? content.sender) = (Some? pt.membership_tag)) then
-    internal_failure "message_plaintext_to_network: membership_tag must be present iff sender = Member"
-  else if not (not (NT.S_member? content.sender) || length (Some?.v pt.membership_tag <: bytes) < pow2 30) then
-    internal_failure "message_plaintext_to_network: membership_tag too long"
-  else (
-    return ({
-      content;
-      auth;
-      membership_tag = if NT.S_member? content.sender then (Some?.v pt.membership_tag) else ();
-    } <: mls_plaintext_nt bytes)
-  )
-
-val network_to_ciphertext_content: #bytes:Type0 -> {|bytes_like bytes|} -> #content_type: content_type_nt -> mls_ciphertext_content_nt bytes content_type -> result (message_ciphertext_content bytes content_type)
-let network_to_ciphertext_content #bytes #bl #content_type ciphertext_content =
-  content <-- network_to_message_bare_content ciphertext_content.data.content;
-  auth <-- network_to_message_auth ciphertext_content.data.auth;
-  return ({
-    content;
-    auth;
-    padding = ciphertext_content.padding;
-  })
-
-val ciphertext_content_to_network: #bytes:Type0 -> {|bytes_like bytes|} -> #content_type: content_type_nt -> message_ciphertext_content bytes content_type -> result (mls_ciphertext_content_nt bytes content_type)
-let ciphertext_content_to_network #bytes #bl #content_type ciphertext_content =
-  content <-- message_bare_content_to_network ciphertext_content.content;
-  auth <-- message_auth_to_network ciphertext_content.auth;
-  return ({
-    data = {
-      content;
-      auth;
-    };
-    padding = ciphertext_content.padding;
-  } <: mls_ciphertext_content_nt bytes content_type)
-
-val network_to_encrypted_sender_data: #bytes:Type0 -> {|bytes_like bytes|} -> mls_sender_data_nt bytes -> encrypted_sender_data_content bytes
-let network_to_encrypted_sender_data #bytes #bl sd =
-  ({
-    leaf_index = sd.leaf_index;
-    generation = sd.generation;
-    reuse_guard = sd.reuse_guard;
-  })
-
-val encrypted_sender_data_to_network: #bytes:Type0 -> {|bytes_like bytes|} -> encrypted_sender_data_content bytes -> result (mls_sender_data_nt bytes)
-let encrypted_sender_data_to_network #bytes #bl sd =
-  if not (sd.leaf_index < pow2 32) then
-    internal_failure "encrypted_sender_data_to_network: leaf_index too big"
-  else if not (sd.generation < pow2 32) then
-    internal_failure "encrypted_sender_data_to_network: generation too big"
-  else
-    return ({
-      leaf_index = sd.leaf_index;
-      generation = sd.generation;
-      reuse_guard = sd.reuse_guard;
-    } <: mls_sender_data_nt bytes)
-
-val network_to_message_ciphertext: #bytes:Type0 -> {|bytes_like bytes|} -> mls_ciphertext_nt bytes -> result (message_ciphertext bytes)
-let network_to_message_ciphertext #bytes #bl ct =
-  return ({
-    group_id = ct.group_id;
-    epoch = ct.epoch;
-    content_type = ct.content_type;
-    authenticated_data = ct.authenticated_data;
-    encrypted_sender_data = ct.encrypted_sender_data;
-    ciphertext = ct.ciphertext;
-  } <: message_ciphertext bytes)
-
-val message_ciphertext_to_network: #bytes:Type0 -> {|bytes_like bytes|} -> message_ciphertext bytes -> result (mls_ciphertext_nt bytes)
-let message_ciphertext_to_network #bytes #bl ct =
-  if not (length ct.group_id < pow2 30) then
-     internal_failure "message_ciphertext_to_network: group_id too long"
-  else if not (ct.epoch < pow2 64) then
-     internal_failure "message_ciphertext_to_network: epoch too big"
-  else if not (length ct.authenticated_data < pow2 30) then
-     internal_failure "message_ciphertext_to_network: authenticated_data too long"
-  else if not (length ct.encrypted_sender_data < pow2 30) then
-     internal_failure "message_ciphertext_to_network: encrypted_sender_data too long"
-  else if not (length ct.ciphertext < pow2 30) then
-     internal_failure "message_ciphertext_to_network: ciphertext too long"
-  else (
-    return ({
-      group_id = ct.group_id;
-      epoch = ct.epoch;
-      content_type = ct.content_type;
-      authenticated_data = ct.authenticated_data;
-      encrypted_sender_data = ct.encrypted_sender_data;
-      ciphertext = ct.ciphertext;
-    } <: mls_ciphertext_nt bytes)
-  )
-
 (*** Authentication ***)
 
 val compute_message_confirmation_tag: #bytes:Type0 -> {|crypto_bytes bytes|} -> bytes -> bytes -> result (lbytes bytes (hmac_length #bytes))
 let compute_message_confirmation_tag #bytes #cb confirmation_key confirmed_transcript_hash =
   hmac_hmac confirmation_key confirmed_transcript_hash
 
-val compute_tbs: #bytes:Type0 -> {|bytes_like bytes|} -> message_content bytes -> option (group_context_nt bytes) -> result (mls_content_tbs_nt bytes)
-let compute_tbs #bytes #bl msg group_context =
-  content <-- message_content_to_network msg;
-  if not ((NT.S_member? content.sender || NT.S_new_member_commit? content.sender) = Some? group_context) then
-    internal_failure "compute_tbs: group_context must be present iff sender is member or new_member"
-  else (
-    return ({
-      wire_format = msg.wire_format;
-      content;
-      group_context = (match group_context with | Some gc -> gc | None -> ());
-    } <: mls_content_tbs_nt bytes)
-  )
+val knows_group_context: #bytes:Type0 -> {|bytes_like bytes|} -> sender_nt bytes -> bool
+let knows_group_context #bytes #bl sender = NT.S_member? sender || NT.S_new_member_commit? sender
 
-val compute_tbm: #bytes:Type0 -> {|bytes_like bytes|} -> message_content bytes -> message_auth bytes -> option (group_context_nt bytes) -> result (mls_content_tbm_nt bytes)
-let compute_tbm #bytes #bl msg auth group_context =
-  tbs <-- compute_tbs msg group_context;
-  auth <-- message_auth_to_network auth;
-  return ({
-    content_tbs = tbs;
+val compute_tbs: #bytes:Type0 -> {|bytes_like bytes|} -> wire_format_nt -> content:mls_content_nt bytes -> group_context:option (group_context_nt bytes){Some? group_context <==> knows_group_context content.sender} -> mls_content_tbs_nt bytes
+let compute_tbs #bytes #bl wire_format content group_context =
+  ({
+    wire_format;
+    content;
+    group_context = (match group_context with | Some gc -> gc | None -> ());
+  } <: mls_content_tbs_nt bytes)
+
+val compute_tbm: #bytes:Type0 -> {|bytes_like bytes|} -> content:mls_content_nt bytes -> mls_content_auth_data_nt bytes content.content.content_type -> group_context:option (group_context_nt bytes){Some? group_context <==> knows_group_context content.sender} -> mls_content_tbm_nt bytes
+let compute_tbm #bytes #bl content auth group_context =
+  let content_tbs = compute_tbs (WF_mls_plaintext ()) content group_context in
+  ({
+    content_tbs;
     auth;
   } <: mls_content_tbm_nt bytes)
 
-val compute_message_signature: #bytes:Type0 -> {|crypto_bytes bytes|} -> sign_private_key bytes -> sign_nonce bytes -> message_content bytes -> option (group_context_nt bytes) -> result (sign_signature bytes)
-let compute_message_signature #bytes #cb sk rand msg group_context =
-  tbs <-- compute_tbs msg group_context;
+val compute_message_signature: #bytes:Type0 -> {|crypto_bytes bytes|} -> sign_private_key bytes -> sign_nonce bytes -> wire_format_nt -> content:mls_content_nt bytes -> group_context:option (group_context_nt bytes){Some? group_context <==> knows_group_context content.sender} -> result (sign_signature bytes)
+let compute_message_signature #bytes #cb sk rand wire_format msg group_context =
+  let tbs = compute_tbs wire_format msg group_context in
   let serialized_tbs = serialize (mls_content_tbs_nt bytes) tbs in
-  sign_with_label sk (string_to_bytes #bytes "MLSPlaintextTBS") serialized_tbs rand
+  sign_with_label sk (string_to_bytes #bytes "MLSContentTBS") serialized_tbs rand
 
-val check_message_signature: #bytes:Type0 -> {|crypto_bytes bytes|} -> sign_public_key bytes -> sign_signature bytes -> message_content bytes -> option (group_context_nt bytes) -> result bool
-let check_message_signature #bytes #cb pk signature msg group_context =
-  tbs <-- compute_tbs msg group_context;
+val check_message_signature: #bytes:Type0 -> {|crypto_bytes bytes|} -> sign_public_key bytes -> sign_signature bytes -> wire_format_nt -> content:mls_content_nt bytes -> group_context:option (group_context_nt bytes){Some? group_context <==> knows_group_context content.sender} -> result bool
+let check_message_signature #bytes #cb pk signature wire_format msg group_context =
+  let tbs = compute_tbs wire_format msg group_context in
   let serialized_tbs = serialize (mls_content_tbs_nt bytes) tbs in
-  verify_with_label pk (string_to_bytes #bytes "MLSPlaintextTBS") serialized_tbs signature
+  verify_with_label pk (string_to_bytes #bytes "MLSContentTBS") serialized_tbs signature
 
-val compute_message_membership_tag: #bytes:Type0 -> {|crypto_bytes bytes|} -> bytes -> message_content bytes -> message_auth bytes -> option (group_context_nt bytes) -> result (lbytes bytes (hmac_length #bytes))
+val compute_message_membership_tag: #bytes:Type0 -> {|crypto_bytes bytes|} -> bytes -> content:mls_content_nt bytes -> mls_content_auth_data_nt bytes content.content.content_type -> group_context:option (group_context_nt bytes){Some? group_context <==> knows_group_context content.sender} -> result (lbytes bytes (hmac_length #bytes))
 let compute_message_membership_tag #bytes #cb membership_key msg auth group_context =
-  tbm <-- compute_tbm msg auth group_context;
+  let tbm = compute_tbm msg auth group_context in
   let serialized_tbm = serialize (mls_content_tbm_nt bytes) tbm in
   hmac_hmac membership_key serialized_tbm
 
+//TODO: this function should be refactored
 val message_compute_auth: #bytes:Type0 -> {|crypto_bytes bytes|} -> message_content bytes -> sign_private_key bytes -> sign_nonce bytes -> option (group_context_nt bytes) -> bytes -> bytes -> result (message_auth bytes)
 let message_compute_auth #bytes #cb msg sk rand group_context confirmation_key interim_transcript_hash =
-  signature <-- compute_message_signature sk rand msg group_context;
-  confirmation_tag <-- (
-    if msg.content_type = CT_commit () then (
-      confirmed_transcript_hash <-- compute_confirmed_transcript_hash msg signature interim_transcript_hash;
-      confirmation_tag <-- compute_message_confirmation_tag confirmation_key confirmed_transcript_hash;
-      return (Some confirmation_tag <: option bytes)
-    ) else (
-      return None
-    )
-  );
-  return ({
-    signature = signature;
-    confirmation_tag = confirmation_tag;
-  } <: message_auth bytes)
+  msg_network <-- message_content_to_network msg;
+  if not (Some? group_context = knows_group_context msg_network.sender) then
+    internal_failure "message_compute_auth: bad optional group context"
+  else (
+    signature <-- compute_message_signature sk rand msg.wire_format msg_network group_context;
+    confirmation_tag <-- (
+      if msg.content_type = CT_commit () then (
+        confirmed_transcript_hash <-- compute_confirmed_transcript_hash msg signature interim_transcript_hash;
+        confirmation_tag <-- compute_message_confirmation_tag confirmation_key confirmed_transcript_hash;
+        return (Some confirmation_tag <: option bytes)
+      ) else (
+        return None
+      )
+    );
+    return ({
+      signature = signature;
+      confirmation_tag = confirmation_tag;
+    } <: message_auth bytes)
+  )
 
 (*** From/to plaintext ***)
 
 //TODO check membership tag
-val message_plaintext_to_message: #bytes:Type0 -> {|bytes_like bytes|} -> message_plaintext bytes -> message_content bytes & message_auth bytes
+val message_plaintext_to_message: #bytes:Type0 -> {|bytes_like bytes|} -> mls_plaintext_nt bytes -> mls_authenticated_content_nt bytes
 let message_plaintext_to_message #bytes #bl pt =
-  (pt.content, pt.auth)
+  {
+    wire_format = WF_mls_plaintext ();
+    content = pt.content;
+    auth = pt.auth;
+  }
 
-val message_to_message_plaintext: #bytes:Type0 -> {|crypto_bytes bytes|} -> membership_key:bytes -> option (group_context_nt bytes) -> (msg:message_content bytes{msg.wire_format == WF_mls_plaintext ()}) * message_auth bytes -> result (message_plaintext bytes)
-let message_to_message_plaintext #bytes #cb membership_key group_context (msg, msg_auth) =
+val message_to_message_plaintext: #bytes:Type0 -> {|crypto_bytes bytes|} -> membership_key:bytes -> auth_msg:mls_authenticated_content_nt bytes{auth_msg.wire_format == WF_mls_plaintext ()} -> group_context:option (group_context_nt bytes){Some? group_context <==> knows_group_context auth_msg.content.sender} -> result (mls_plaintext_nt bytes)
+let message_to_message_plaintext #bytes #cb membership_key auth_msg group_context =
   membership_tag <-- (
-    match msg.sender with
-    | S_member _ -> (
-      res <-- compute_message_membership_tag membership_key msg msg_auth group_context;
-      return (Some (res <: bytes))
+    match auth_msg.content.sender with
+    | NT.S_member _ -> (
+      res <-- compute_message_membership_tag membership_key auth_msg.content auth_msg.auth group_context;
+      return (res <: membership_tag_nt bytes auth_msg.content.sender)
     )
-    | _ -> return None
+    | _ -> return ()
   );
   return ({
-    content = msg;
-    auth = msg_auth;
+    content = auth_msg.content;
+    auth = auth_msg.auth;
     membership_tag;
-  } <: message_plaintext bytes)
+  } <: mls_plaintext_nt bytes)
 
 (*** From/to ciphertext ***)
 
@@ -245,34 +115,23 @@ let get_ciphertext_sample #bytes #cb ct =
   else
     fst (unsafe_split ct len)
 
-val message_ciphertext_to_sender_data_aad: #bytes:Type0 -> {|bytes_like bytes|} -> message_ciphertext bytes -> result (mls_sender_data_aad_nt bytes)
+//Used in decryption
+val message_ciphertext_to_sender_data_aad: #bytes:Type0 -> {|bytes_like bytes|} -> mls_ciphertext_nt bytes -> mls_sender_data_aad_nt bytes
 let message_ciphertext_to_sender_data_aad #bytes #bl ct =
-  if not (length ct.group_id < pow2 30) then (
-    internal_failure "message_ciphertext_to_sender_data_aad: group_id too long"
-  ) else if not (ct.epoch < pow2 64) then (
-    internal_failure "message_ciphertext_to_sender_data_aad: epoch too big"
-  ) else (
-    return ({
-      group_id = ct.group_id;
-      epoch = ct.epoch;
-      content_type = ct.content_type;
-    } <: mls_sender_data_aad_nt bytes)
-  )
+  ({
+    group_id = ct.group_id;
+    epoch = ct.epoch;
+    content_type = ct.content_type;
+  } <: mls_sender_data_aad_nt bytes)
 
-//TODO (?): copy-pasted from above
-val message_to_sender_data_aad: #bytes:Type0 -> {|bytes_like bytes|} -> message_content bytes -> result (mls_sender_data_aad_nt bytes)
-let message_to_sender_data_aad #bytes #bl ct =
-  if not (length ct.group_id < pow2 30) then (
-    internal_failure "message_to_sender_data_aad: group_id too long"
-  ) else if not (ct.epoch < pow2 30) then (
-    internal_failure "message_to_sender_data_aad: epoch too big"
-  ) else (
-    return ({
-      group_id = ct.group_id;
-      epoch = ct.epoch;
-      content_type = ct.content_type;
-    } <: mls_sender_data_aad_nt bytes)
-  )
+//Used in encryption
+val message_to_sender_data_aad: #bytes:Type0 -> {|bytes_like bytes|} -> mls_content_nt bytes -> mls_sender_data_aad_nt bytes
+let message_to_sender_data_aad #bytes #bl content =
+  ({
+    group_id = content.group_id;
+    epoch = content.epoch;
+    content_type = content.content.content_type;
+  } <: mls_sender_data_aad_nt bytes)
 
 val decrypt_sender_data: #bytes:Type0 -> {|crypto_bytes bytes|} -> mls_sender_data_aad_nt bytes -> ciphertext_sample:bytes -> sender_data_secret:bytes -> encrypted_sender_data:bytes -> result (mls_sender_data_nt bytes)
 let decrypt_sender_data #bytes #cb ad ciphertext_sample sender_data_secret encrypted_sender_data =
@@ -287,45 +146,30 @@ let encrypt_sender_data #bytes #cb ad ciphertext_sample sender_data_secret sende
   sender_data_nonce <-- expand_with_label sender_data_secret (string_to_bytes #bytes "nonce") ciphertext_sample (aead_nonce_length #bytes);
   aead_encrypt sender_data_key sender_data_nonce (serialize (mls_sender_data_aad_nt bytes) ad) (serialize (mls_sender_data_nt bytes) sender_data)
 
-val message_ciphertext_to_ciphertext_content_aad: #bytes:Type0 -> {|bytes_like bytes|} -> ct:message_ciphertext bytes -> result (res:mls_ciphertext_content_aad_nt bytes{res.content_type == ct.content_type})
+// Used in decryption
+val message_ciphertext_to_ciphertext_content_aad: #bytes:Type0 -> {|bytes_like bytes|} -> ct:mls_ciphertext_nt bytes -> res:mls_ciphertext_content_aad_nt bytes{res.content_type == ct.content_type}
 let message_ciphertext_to_ciphertext_content_aad #bytes #bl ct =
-  if not (length ct.group_id < pow2 30) then (
-    internal_failure "message_ciphertext_to_ciphertext_content_aad: group_id too long"
-  ) else if not (ct.epoch < pow2 64) then (
-    internal_failure "message_ciphertext_to_ciphertext_content_aad: epoch too big"
-  ) else if not (length ct.authenticated_data < pow2 30) then (
-    internal_failure "message_ciphertext_to_ciphertext_content_aad: authenticated_data too long"
-  ) else (
-    return ({
-      group_id = ct.group_id;
-      epoch = ct.epoch;
-      content_type = ct.content_type;
-      authenticated_data = ct.authenticated_data;
-    } <: mls_ciphertext_content_aad_nt bytes)
-  )
+  ({
+    group_id = ct.group_id;
+    epoch = ct.epoch;
+    content_type = ct.content_type;
+    authenticated_data = ct.authenticated_data;
+  } <: mls_ciphertext_content_aad_nt bytes)
 
 val decrypt_ciphertext_content: #bytes:Type0 -> {|crypto_bytes bytes|} -> ad:mls_ciphertext_content_aad_nt bytes -> aead_key bytes -> aead_nonce bytes -> ct:bytes -> result (mls_ciphertext_content_nt bytes ad.content_type)
 let decrypt_ciphertext_content #bytes #cb ad key nonce ct =
   ciphertext_content <-- aead_decrypt key nonce (serialize (mls_ciphertext_content_aad_nt bytes) ad) ct;
   from_option "decrypt_ciphertext_content: malformed ciphertext content" (parse (mls_ciphertext_content_nt bytes ad.content_type) ciphertext_content)
 
-//TODO (?): copy-pasted from message_ciphertext_to_ciphertext_content_aad, can we simplify?
-val message_to_ciphertext_content_aad: #bytes:Type0 -> {|bytes_like bytes|} -> msg:message_content bytes -> result (res:mls_ciphertext_content_aad_nt bytes{res.content_type == msg.content_type})
-let message_to_ciphertext_content_aad #bytes #bl msg =
-  if not (length msg.group_id < pow2 30) then (
-    internal_failure "message_to_ciphertext_content_aad: group_id too long"
-  ) else if not (msg.epoch < pow2 64) then (
-    internal_failure "message_to_ciphertext_content_aad: epoch too big"
-  ) else if not (length msg.authenticated_data < pow2 30) then (
-    internal_failure "message_to_ciphertext_content_aad: authenticated_data too long"
-  ) else (
-    return ({
-      group_id = msg.group_id;
-      epoch = msg.epoch;
-      content_type = msg.content_type;
-      authenticated_data = msg.authenticated_data;
-    } <: mls_ciphertext_content_aad_nt bytes)
-  )
+// Used in encryption
+val message_to_ciphertext_content_aad: #bytes:Type0 -> {|bytes_like bytes|} -> content:mls_content_nt bytes -> res:mls_ciphertext_content_aad_nt bytes{res.content_type == content.content.content_type}
+let message_to_ciphertext_content_aad #bytes #bl content =
+  ({
+    group_id = content.group_id;
+    epoch = content.epoch;
+    content_type = content.content.content_type;
+    authenticated_data = content.authenticated_data;
+  } <: mls_ciphertext_content_aad_nt bytes)
 
 val encrypt_ciphertext_content: #bytes:Type0 -> {|crypto_bytes bytes|} -> ad:mls_ciphertext_content_aad_nt bytes -> aead_key bytes -> aead_nonce bytes -> (mls_ciphertext_content_nt bytes ad.content_type) -> result bytes
 let encrypt_ciphertext_content #bytes #cb ad key nonce pt =
@@ -339,12 +183,11 @@ let apply_reuse_guard #bytes #cb reuse_guard nonce =
   let new_nonce_head = xor nonce_head reuse_guard in
   concat #bytes new_nonce_head nonce_tail
 
-val message_ciphertext_to_message: #bytes:Type0 -> {|crypto_bytes bytes|} -> l:nat -> encryption_secret:bytes -> sender_data_secret:bytes -> message_ciphertext bytes -> result (message_content bytes & message_auth bytes)
+val message_ciphertext_to_message: #bytes:Type0 -> {|crypto_bytes bytes|} -> l:nat -> encryption_secret:bytes -> sender_data_secret:bytes -> mls_ciphertext_nt bytes -> result (mls_authenticated_content_nt bytes)
 let message_ciphertext_to_message #bytes #cb l encryption_secret sender_data_secret ct =
   sender_data <-- (
-    sender_data_ad <-- message_ciphertext_to_sender_data_aad ct;
-    sender_data <-- decrypt_sender_data sender_data_ad (get_ciphertext_sample ct.ciphertext) sender_data_secret ct.encrypted_sender_data;
-    return (network_to_encrypted_sender_data sender_data)
+    let sender_data_ad = message_ciphertext_to_sender_data_aad ct in
+    decrypt_sender_data sender_data_ad (get_ciphertext_sample ct.ciphertext) sender_data_secret ct.encrypted_sender_data
   );
   rs_output <-- (
     sender_index <-- (
@@ -365,58 +208,74 @@ let message_ciphertext_to_message #bytes #cb l encryption_secret sender_data_sec
     let nonce = rs_output.nonce in
     let key = rs_output.key in
     let patched_nonce = apply_reuse_guard sender_data.reuse_guard nonce in
-    ciphertext_content_ad <-- message_ciphertext_to_ciphertext_content_aad ct;
-    ciphertext_content_network <-- decrypt_ciphertext_content ciphertext_content_ad key patched_nonce ct.ciphertext;
-    network_to_ciphertext_content (ciphertext_content_network <: mls_ciphertext_content_nt bytes ct.content_type)
+    let ciphertext_content_ad = message_ciphertext_to_ciphertext_content_aad ct in
+    decrypt_ciphertext_content ciphertext_content_ad key patched_nonce ct.ciphertext
   );
-  return (({
+  return ({
     wire_format = WF_mls_ciphertext ();
-    group_id = ct.group_id;
-    epoch = ct.epoch;
-    sender = S_member sender_data.leaf_index;
-    authenticated_data = ct.authenticated_data;
-    content_type = ct.content_type;
-    content = ciphertext_content.content;
-  } <: message_content bytes), ({
-    signature = ciphertext_content.auth.signature;
-    confirmation_tag = ciphertext_content.auth.confirmation_tag;
-  } <: message_auth bytes))
+    content = {
+      group_id = ct.group_id;
+      epoch = ct.epoch;
+      sender = NT.S_member sender_data.leaf_index;
+      authenticated_data = ct.authenticated_data;
+      content = {
+        content_type = ct.content_type;
+        content = ciphertext_content.data.content;
+      };
+    };
+    auth = {
+      signature = ciphertext_content.data.auth.signature;
+      confirmation_tag = ciphertext_content.data.auth.confirmation_tag;
+    };
+  } <: mls_authenticated_content_nt bytes)
 
-val message_to_message_ciphertext: #bytes:Type0 -> {|crypto_bytes bytes|} -> ratchet_state bytes -> lbytes bytes 4 -> bytes -> (msg:message_content bytes{msg.wire_format == WF_mls_ciphertext ()} * message_auth bytes) -> result (message_ciphertext bytes & ratchet_state bytes)
-let message_to_message_ciphertext #bytes #cb ratchet reuse_guard sender_data_secret (msg, msg_auth) =
+val get_serializeable_bytes: #bytes:Type0 -> {|bytes_like bytes|} -> bytes -> result (mls_bytes bytes)
+let get_serializeable_bytes #bytes #bl b =
+  if not (length b < pow2 30) then (
+    internal_failure "get_serializeable_bytes: buffer too long"
+  ) else (
+    return b
+  )
+
+val message_to_message_ciphertext: #bytes:Type0 -> {|crypto_bytes bytes|} -> ratchet_state bytes -> lbytes bytes 4 -> bytes -> msg:mls_authenticated_content_nt bytes{msg.wire_format == WF_mls_ciphertext ()} -> result (mls_ciphertext_nt bytes & ratchet_state bytes)
+let message_to_message_ciphertext #bytes #cb ratchet reuse_guard sender_data_secret auth_msg =
   ciphertext <-- (
     key_nonce <-- ratchet_get_key ratchet;
     let key = key_nonce.key in
     let patched_nonce = apply_reuse_guard reuse_guard key_nonce.nonce in
-    let ciphertext_content: message_ciphertext_content bytes (msg.content_type) = {
-      content = msg.content;
-      auth = msg_auth;
+    let ciphertext_content: mls_ciphertext_content_nt bytes (auth_msg.content.content.content_type) = {
+      data = {
+        content = auth_msg.content.content.content;
+        auth = auth_msg.auth;
+      };
       padding = []; //TODO
     } in
-    ciphertext_content_network <-- ciphertext_content_to_network ciphertext_content;
-    ciphertext_content_ad <-- message_to_ciphertext_content_aad msg;
-    encrypt_ciphertext_content ciphertext_content_ad key patched_nonce ciphertext_content_network
+    let ciphertext_content_ad = message_to_ciphertext_content_aad auth_msg.content in
+    ciphertext <-- encrypt_ciphertext_content ciphertext_content_ad key patched_nonce ciphertext_content;
+    get_serializeable_bytes ciphertext
   );
   encrypted_sender_data <-- (
-    if not (S_member? msg.sender) then
+    if not (NT.S_member? auth_msg.content.sender) then
       error "message_to_message_ciphertext: sender is not a member"
+    else if not (ratchet.generation < pow2 32) then
+      internal_failure "message_to_message_ciphertext: ratchet too big"
     else (
-      sender_data_ad <-- message_to_sender_data_aad msg;
+      let sender_data_ad = message_to_sender_data_aad auth_msg.content in
       let sender_data = ({
-        leaf_index = S_member?.leaf_index msg.sender;
+        leaf_index = NT.S_member?.leaf_index auth_msg.content.sender;
         generation = ratchet.generation;
         reuse_guard = reuse_guard;
       }) in
-      sender_data_network <-- encrypted_sender_data_to_network sender_data;
-      encrypt_sender_data sender_data_ad (get_ciphertext_sample ciphertext) sender_data_secret sender_data_network
+      encrypted_sender_data <-- encrypt_sender_data sender_data_ad (get_ciphertext_sample ciphertext) sender_data_secret sender_data;
+      get_serializeable_bytes encrypted_sender_data
     )
   );
   new_ratchet <-- ratchet_next_state ratchet;
-  return ({
-    group_id = msg.group_id;
-    epoch = msg.epoch;
-    content_type = msg.content_type;
-    authenticated_data = msg.authenticated_data;
+  return (({
+    group_id = auth_msg.content.group_id;
+    epoch = auth_msg.content.epoch;
+    content_type = auth_msg.content.content.content_type;
+    authenticated_data = auth_msg.content.authenticated_data;
     encrypted_sender_data = encrypted_sender_data;
     ciphertext = ciphertext;
-  }, new_ratchet)
+  } <: mls_ciphertext_nt bytes), new_ratchet)
